wip

pulse/lib/steel/pulse/Pulse.Checker.Auto.Util.fsti
@@ -76,124 +76,695 @@ let ghost_comp pre post =
 
 open Pulse.Checker.VPropEquiv
 
+val dom_env (g:env) : Set.set var
+type typ = term
+
+type uvs_t = Map.t var typ
+type substitution (g0:env) (uvs:uvs_t) =
+  m:Map.t var term {
+    forall (x:var). Map.contains m x ==>
+                    (Map.contains uvs x /\
+                     tot_typing g0 (Map.sel m x) (Map.sel uvs x))
+  }
+
+val apply_ss (#g0:_) (#uvs:_) (s:substitution g0 uvs) (t:term) : term
+val apply_ss_st (#g0:_) (#uvs:_) (s:substitution g0 uvs) (t:st_term) : st_term
+val apply_c (#g0:_) (#uvs:_) (s:substitution g0 uvs) (c:comp) : comp
+
+let uvars (t:term) (uvs:uvs_t) : Set.set var =
+  Set.intersect (freevars t) (Map.domain uvs)
+let uvars_st (t:st_term) (uvs:uvs_t) : Set.set var =
+  Set.intersect (freevars_st t) (Map.domain uvs)
+
 //
 // This remains fixed as prover state is transformed by steps
 //
 noeq
-type prover_state_preamble (g:env) = {
+type prover_state_preamble = {
+  g0:env;
+  g:env;
   ctxt:vprop;
-  ctxt_typing:vprop_typing g ctxt;
+  ctxt_typing:vprop_typing g0 ctxt;
   t:st_term;
   c:comp_st;
   t_typing:st_typing g t c;
 }
 
+val env_contains (g:env) (x:var) (t:typ) : prop
+
+let set_difference (#a:eqtype) (s1 s2:Set.set a) =
+  Set.intersect s1 (Set.complement s2)
+
+let uvs_invariant (g0 g:env) (uvs:uvs_t) : prop =
+  g `env_extends` g0 /\
+  Set.equal (set_difference (dom_env g) (dom_env g0)) (Map.domain uvs) /\
+  (forall (x:var). Map.contains uvs x ==>
+                   env_contains g x (Map.sel uvs x))
+
 noeq
-type prover_state (g:env) (preamble:prover_state_preamble g) = {
-  (* the in-progress proof state *)
-  matched_pre:term; (* conjuncts that we have already derived *)
-  unmatched_pre:list term; (* conjuncts remaining to be derived *)
-  remaining_ctxt:list term; (* unused conjuncts in the context *)
-  (* Ghost proof steps witnessing the derivation of matched_pre from ctxt *)
-  proof_steps: st_term;
-  proof_steps_typing:
-    st_typing g
-      proof_steps
-      (ghost_comp preamble.ctxt (Tm_Star (list_as_vprop remaining_ctxt) matched_pre));
-  pre_equiv:
-    vprop_equiv g
+type prover_state (preamble:prover_state_preamble) = {
+  matched:term;
+  unmatched:list term;
+  remaining:list term;
+  steps:st_term;
+
+  uvs:uvs_t;
+  ss:substitution preamble.g0 uvs;
+
+  remaining_typing:vprop_typing preamble.g0 (list_as_vprop remaining);
+
+  unmatched_typing:vprop_typing preamble.g (list_as_vprop unmatched);
+
+  steps_typing:st_typing preamble.g0 steps
+    (ghost_comp
+       preamble.ctxt
+       (Tm_Star (list_as_vprop remaining) (apply_ss ss matched)));
+
+  veq:vprop_equiv preamble.g (comp_pre preamble.c)
+                             (Tm_Star (list_as_vprop unmatched) matched);
+
+  props:squash (
+    uvs_invariant preamble.g0 preamble.g uvs /\
+    uvars matched uvs `Set.subset` Map.domain ss
+  );
+}
+
+let ss_extends (#g0:_) (#uvs:_) (ss1 ss2:substitution g0 uvs) : prop =
+  forall (x:var). (Map.contains ss2 x ==> Map.contains ss1 x) /\
+                  (Map.sel ss1 x == Map.sel ss2 x)
+
+val apply_ss_uvars (#g0:_) (#uvs:_) (ss:substitution g0 uvs) (t:term)
+  : Lemma (uvars (apply_ss ss t) uvs ==
+           set_difference (uvars t uvs) (Map.domain ss))
+
+val apply_ss_st_uvars (#g0:_) (#uvs:_) (ss:substitution g0 uvs) (t:st_term)
+  : Lemma (uvars_st (apply_ss_st ss t) uvs ==
+           set_difference (uvars_st t uvs) (Map.domain ss))
+
+val apply_ss_star (#g0:_) (#uvs:_) (ss:substitution g0 uvs) (p1 p2:vprop)
+  : Lemma (apply_ss ss (Tm_Star p1 p2) == apply_ss ss p1 `Tm_Star` apply_ss ss p2)
+
+val extends_apply (#g0:_) (#uvs:_) (ss1 ss2:substitution g0 uvs) (t:term)
+  : Lemma
+      (requires
+         ss1 `ss_extends` ss2 /\
+         uvars t uvs `Set.subset` Map.domain ss2)
+      (ensures apply_ss ss1 t == apply_ss ss2 t)
+
+val extends_apply_st (#g0:_) (#uvs:_) (ss1 ss2:substitution g0 uvs) (t:st_term)
+  : Lemma
+      (requires
+         ss1 `ss_extends` ss2 /\
+         uvars_st t uvs `Set.subset` Map.domain ss2)
+      (ensures apply_ss_st ss1 t == apply_ss_st ss2 t)
+
+
+val typing_ss (#g0:_) (#uvs:_) (g:env) (t:st_term) (c:comp) (t_typing:st_typing g t c) (ss:substitution g0 uvs)
+  : Pure (st_typing g (apply_ss_st ss t) (apply_c ss c))
+         (requires uvs_invariant g0 g uvs)
+         (ensures fun _ -> True)
+
+val veq_ss (#g0:_) (#uvs:_) (g:env) (p1 p2:vprop) (veq:vprop_equiv g p1 p2) (ss:substitution g0 uvs)
+  : Pure (vprop_equiv g (apply_ss ss p1) (apply_ss ss p2))
+         (requires uvs_invariant g0 g uvs)
+         (ensures fun _ -> True)
+
+val veq_weakening (#g:_) (#p1 #p2:_) (veq:vprop_equiv g p1 p2) (g':env { env_extends g' g })
+  : vprop_equiv g' p1 p2
+
+val st_typing_strengthening (#g:_) (#t:st_term) (#c:comp_st) (t_typing:st_typing g t c)
+  (g':env { env_extends g g' })
+  : Pure (st_typing g' t c)
+         (requires
+            freevars_st t `Set.subset` dom_env g' /\
+            freevars_comp c `Set.subset` dom_env g')
+         (ensures fun _ -> True)
+
+val tot_typing_strengthening (#g:_) (#t:term) (#ty:term) (t_typing:tot_typing g t ty)
+  (g':env { env_extends g g' })
+  : Pure (tot_typing g' t ty)
+         (requires
+            freevars t `Set.subset` dom_env g' /\
+            freevars ty `Set.subset` dom_env g')
+         (ensures fun _ -> True)
+
+val veq_strengthening (#g:_) (#p1 #p2:_) (veq:vprop_equiv g p1 p2)
+  (g':env { env_extends g g' })
+  : Pure (vprop_equiv g' p1 p2)
+         (requires
+            freevars p1 `Set.subset` dom_env g' /\
+            freevars p2 `Set.subset` dom_env g')
+         (ensures fun _ -> True)
+
+let with_pre_post (c:comp_st) (pre:vprop) (post:vprop) : comp_st =
+  match c with
+  | C_ST s
+  | C_STGhost _ s
+  | C_STAtomic _ s -> with_st_comp c { s with pre; post }
+
+val pre_post_equiv (#g:env) (#t:st_term) (#c:comp_st {ln (comp_post c)})
+  (d:st_typing g t c)
+  (#pre:vprop) (_:vprop_equiv g (comp_pre c) pre)
+  (#post:vprop) (_:vprop_equiv g (comp_post c) post)
+  : c':comp_st { c' == with_pre_post c pre post } &
+    st_typing g t c'
+
+type prover_t =
+  #(preamble:_) ->
+  p:prover_state preamble ->
+  T.Tac (option (p':prover_state preamble { p'.unmatched == [] /\
+                                            p'.uvs == p.uvs /\
+                                            p'.ss `ss_extends` p.ss }))
+
+type prover_step =
+  #(preamble:_) ->
+  p:prover_state preamble ->
+  prover:prover_t ->
+  T.Tac (option (p':prover_state preamble { p'.uvs == p.uvs /\
+                                            p'.ss `ss_extends` p.ss }))
+
+
+let idem_steps (g:env) (ctxt:vprop)
+  : t:st_term { freevars_st t == Set.empty } &
+    st_typing g t (ghost_comp ctxt (Tm_Star (list_as_vprop (vprop_as_list ctxt))
+                                            Tm_Emp)) = magic ()
+
+val empty_uvs : uvs_t
+val empty_ss (g0:_) : substitution g0 empty_uvs
+
+val vprop_as_list_of_list_as_vprop (l:list vprop)
+  : Lemma (vprop_as_list (list_as_vprop l) == l)
+          [SMTPat (vprop_as_list (list_as_vprop l))]
+
+val list_as_vprop_of_vprop_as_list (p:vprop)
+  : Lemma (list_as_vprop (vprop_as_list p) == p)
+          [SMTPat (list_as_vprop (vprop_as_list p))]
+
+let prove_precondition (#g:env) (#ctxt:term) (ctxt_typing:tot_typing g ctxt Tm_VProp)
+  (#t:st_term) (#c:comp_st) (t_typing:st_typing g t c)
+  (prover:prover_t)
+  : T.Tac (option (t:st_term &
+                   c:comp_st { comp_pre c == ctxt } &
+                   st_typing g t c)) =
+  
+  let preamble = {
+    g0 = g;
+    g;
+    ctxt;
+    ctxt_typing;
+    t;
+    c;
+    t_typing
+  } in
+
+  let (| steps, steps_typing |) = idem_steps g ctxt in
+
+  let matched = Tm_Emp in
+  let unmatched = vprop_as_list (comp_pre c) in
+  let remaining = vprop_as_list ctxt in
+  let steps = steps in
+  let uvs = empty_uvs in
+  let ss = empty_ss g in
+
+  assume (apply_ss ss matched == Tm_Emp);
+  let (| steps, steps_typing |) = idem_steps g ctxt in
+  let steps_typing : st_typing preamble.g steps
+    (ghost_comp preamble.ctxt (Tm_Star (list_as_vprop remaining) (apply_ss ss matched))) = steps_typing in
+
+  let veq : vprop_equiv preamble.g (comp_pre preamble.c)
+                                   (Tm_Star (list_as_vprop unmatched) matched) = magic () in
+
+  assume (Map.domain empty_uvs == Set.empty);
+  assume (g `env_extends` g);
+
+
+  let p = {
+    matched;
+    unmatched;
+    remaining;
+    steps;
+    uvs;
+    ss;
+    remaining_typing = ctxt_typing;
+    unmatched_typing = magic ();  // get it from inversion of t_typing
+    steps_typing; veq; props = ();
+  } in
+
+  let popt = prover p in
+  match popt with
+  | Some p' ->
+    let steps_typing : st_typing g p'.steps
+      (ghost_comp ctxt (Tm_Star (list_as_vprop p'.remaining)
+                                (apply_ss p'.ss p'.matched))) = p'.steps_typing in
+    assert (Set.equal (Map.domain p'.ss) Set.empty);
+    // since substitution is empty
+    assume (apply_ss p'.ss p'.matched == p'.matched);
+    let steps_typing : st_typing g p'.steps
+      (ghost_comp ctxt (Tm_Star (list_as_vprop p'.remaining) p'.matched)) = steps_typing in
+
+    let veq : vprop_equiv g (comp_pre c)
+                            (Tm_Star (list_as_vprop []) p'.matched) = p'.veq in
+    // replacing list_as_vprop [] with Tm_Emp and then normalizing star
+    let veq : vprop_equiv g (comp_pre c) p'.matched = magic () in
+
+    // use veq with steps_typing
+    let steps_typing : st_typing g p'.steps
+      (ghost_comp ctxt (Tm_Star (list_as_vprop p'.remaining) (comp_pre c))) = magic () in
+
+    // we can now bind p'.steps with c
+
+    admit ()
+  | None -> None
+
+val try_match (#g0:_) (#uvs:_)
+  (unm:vprop)
+  (rem:vprop)
+  (ss:substitution g0 uvs)
+  : T.Tac (option (ss':substitution g0 uvs { ss' `ss_extends` ss /\
+                                             freevars unm `Set.subset` Map.domain ss' } &
+                   vprop_equiv g0 (apply_ss ss' unm) rem))
+
+
+let coerce_eq (#a #b:Type) (x:a) (_:squash (a == b)) : y:b { y === x } = x
+
+let match_step (#preamble:_) (p:prover_state preamble)
+  (unm:vprop)
+  (unmatched':list vprop)
+  (rem:vprop)
+  (remaining':list vprop)
+  (veq_unm:vprop_equiv preamble.g (list_as_vprop p.unmatched) (Tm_Star unm (list_as_vprop unmatched')))
+  (veq_rem:vprop_equiv preamble.g (list_as_vprop p.remaining) (Tm_Star rem (list_as_vprop remaining')))
+
+  : T.Tac (option (p':prover_state preamble { p'.uvs == p.uvs /\
+                                              p'.ss `ss_extends` p.ss })) =
+
+  let ropt = try_match unm rem p.ss in
+  match ropt with
+  | Some (| ss', veq_unm_rem |) ->
+    let matched = Tm_Star unm p.matched in
+    let unmatched = unmatched' in
+    let remaining = remaining' in
+
+    let ss = ss' in
+
+    ///// restore p.steps_typing /////
+    extends_apply ss p.ss p.matched;
+    let steps_typing : st_typing preamble.g0 p.steps
+      (ghost_comp preamble.ctxt
+         (Tm_Star (list_as_vprop p.remaining) (apply_ss ss p.matched))) =
+      coerce_eq p.steps_typing () in
+    // some star rearrangement
+    let veq: vprop_equiv preamble.g0
+      (Tm_Star (list_as_vprop p.remaining) (apply_ss ss p.matched))
+      (Tm_Star (list_as_vprop remaining) (Tm_Star rem (apply_ss ss p.matched))) = magic () in
+    let veq_unm_rem : vprop_equiv preamble.g0 (apply_ss ss unm) rem =
+      veq_unm_rem in
+    let veq : vprop_equiv preamble.g0
+      (Tm_Star (list_as_vprop p.remaining) (apply_ss ss p.matched))
+      (Tm_Star (list_as_vprop remaining) (Tm_Star (apply_ss ss unm) (apply_ss ss p.matched))) =
+      magic () in
+    apply_ss_star ss unm p.matched;
+    let veq : vprop_equiv preamble.g0
+      (Tm_Star (list_as_vprop p.remaining) (apply_ss ss p.matched))
+      (Tm_Star (list_as_vprop remaining) (apply_ss ss (Tm_Star unm p.matched))) = veq in
+    let veq_pre : vprop_equiv preamble.g0 preamble.ctxt preamble.ctxt = magic () in
+    assume (ln (Tm_Star (list_as_vprop p.remaining) (apply_ss ss p.matched)));
+    let (| _, steps_typing |) : x:_ & st_typing preamble.g0 p.steps
+      (ghost_comp preamble.ctxt
+         (Tm_Star (list_as_vprop remaining) (apply_ss ss matched))) =
+      pre_post_equiv steps_typing veq_pre veq in
+    /////
+
+    ///// restore p.veq /////
+    let veq : vprop_equiv preamble.g
       (comp_pre preamble.c)
-      (Tm_Star (list_as_vprop unmatched_pre) matched_pre);
-}
+      (Tm_Star (list_as_vprop p.unmatched) p.matched) =
+      p.veq in
+    // use veq_unm
+    let veq : vprop_equiv preamble.g
+      (comp_pre preamble.c)
+      (Tm_Star (Tm_Star unm (list_as_vprop unmatched)) p.matched) = magic () in
+    // stars rearrangement
+    let veq : vprop_equiv preamble.g
+      (comp_pre preamble.c)
+      (Tm_Star (list_as_vprop unmatched) matched) = magic () in
+    /////
 
-let proof_steps_post (#g:_) (#preamble:_) (p:prover_state g preamble) : vprop =
-  Tm_Star (list_as_vprop p.remaining_ctxt) p.matched_pre
+    Some { p with
+           matched;
+           unmatched;
+           remaining;
+           steps = p.steps;
+           uvs = p.uvs;
+           ss;
+           remaining_typing = magic ();  // remaining and matched are sub vprops of original ones,
+                                         // whose typing came in with the orignal prover state
+           unmatched_typing = magic ();
+           steps_typing;
+           veq;
+           props = (); }
+  
+  | _ -> admit ()
 
-let bind_proof_steps_with (#g:env) (#preamble:_) (p:prover_state g preamble)
-  (t:st_term)
-  (c:comp_st {comp_pre c == proof_steps_post p})
-  (t_typing:st_typing g t c)
-  : (t':st_term & st_typing g t' (comp_st_with_pre c preamble.ctxt))
-  = admit()
+module RT = FStar.Reflection.Typing
 
-type prover_step_t =
-  #g:_ ->
-  #preamble:_ ->
-  p:prover_state g preamble ->
-  T.Tac (option (prover_state g preamble))
+val subset_bool (#a:eqtype) (s1 s2:Set.set a)
+  : Tot (b:bool { b ==> Set.subset s1 s2 })
 
-//
-// result of an intro (pure, exists, rewrite) step
-//   that consumes some vprop v from p.unmatched_pre
-//
+#push-options "--z3rlimit_factor 4 --ifuel 1 --fuel 1"
+let intro_exists_step (#preamble:_) (p:prover_state preamble)
+  (u:universe) (t:term) (body:vprop)
+  (unmatched':list vprop)
+  (_:squash (p.unmatched == (Tm_ExistsSL u t body)::unmatched'))
+  
+  //
+  // CHEATING:
+  //   This is a Tac function, but with that calling it in the body
+  //   makes verification time unbearable for fast development
+  //
+  // See comment below in the body
+  //
+  (prover:(#(preamble:_) ->
+           p:prover_state preamble ->
+           (option (p':prover_state preamble { p'.unmatched == [] /\
+                                               p'.uvs == p.uvs /\
+                                               p'.ss `ss_extends` p.ss }))))
 
-let intro_comp (c:comp) =
-  C_STGhost? c /\ comp_u c == u_zero /\ comp_res c == tm_unit
+  : T.Tac (option (p':prover_state preamble { p'.uvs == p.uvs /\
+                                              p'.ss `ss_extends` p.ss })) =
+  
+  let y = fresh preamble.g in
+  let g' = extend y (Inl t) preamble.g in
+  assume (g' `env_extends` preamble.g);
 
-//
-// A proof step that provides v, eating away some of the ctxt
-//
-noeq
-type proof_step (g:env) (ctxt:list vprop) (v:vprop) = {
-  remaining' : list vprop;
+  //// create a sub prover preamble ////
+  let g0_sub = preamble.g0 in
+  let g_sub = g' in
+  let ctxt_sub = list_as_vprop p.remaining in
+  let ctxt_typing_sub : vprop_typing g0_sub (list_as_vprop p.remaining) =
+    p.remaining_typing in
+  let witness_tm = tm_var {
+    nm_index = y;
+    nm_ppname = RT.pp_name_default;
+    nm_range = Range.range_0
+  } in
+  // what should erased be?
+  let t_sub = wr (Tm_IntroExists {
+    erased = false;
+    p = Tm_ExistsSL u t body;
+    witnesses = [witness_tm];
+    should_check = should_check_true
+  }) in
+  let c_sub = comp_intro_exists u t body witness_tm in
+  // the t and Tm_ExistsSL should come from typing of matched
+  // and some inversions
+  let t_typing_sub : st_typing g' t_sub c_sub =
+    T_IntroExists g' u t body witness_tm
+      (magic ())  // typing of t
+      (magic ())  // typing of Tm_ExistsSL
+      (magic ())  // typing of witness_tm
+  in
 
-  t' : st_term;
-  c' : c:comp { intro_comp c /\ comp_post c == v };
-  t'_typing : st_typing g t' c';
+  let preamble_sub = {
+    g0 = g0_sub;
+    g = g_sub;
+    ctxt = ctxt_sub;
+    ctxt_typing = ctxt_typing_sub;
+    t = t_sub;
+    c = c_sub;
+    t_typing = t_typing_sub;
+  } in
+  /////
 
-  remaining_equiv : vprop_equiv g (list_as_vprop ctxt)
-                                  (Tm_Star (comp_pre c') (list_as_vprop remaining'));
-}
+  //// create a sub prover state /////
+  let matched_sub = Tm_Emp in
+  let unmatched_sub = vprop_as_list (comp_pre preamble_sub.c) in
+  let remaining_sub = p.remaining in
 
-// An intro step that makes progress by solving one conjunct
-// v from the p.unmatched_pre
-noeq
-type intro_from_unmatched_step (#g:env) (#preamble:_) (p:prover_state g preamble) = {
-  v : vprop;
+  let remaining_typing:vprop_typing preamble_sub.g0 (list_as_vprop remaining_sub) =
+    p.remaining_typing in
 
-  ps:proof_step g p.remaining_ctxt v;
+  // get from inversion of t_typing_sub
+  let unmatched_typing:vprop_typing preamble_sub.g (list_as_vprop unmatched_sub) =
+    magic () in
+  
+  let (| steps_sub, steps_typing_sub |) = idem_steps preamble_sub.g0 preamble_sub.ctxt in
+  assume (apply_ss p.ss Tm_Emp == Tm_Emp);
+  assume (list_as_vprop (vprop_as_list preamble_sub.ctxt) == preamble_sub.ctxt);
+  let steps_typing_sub : st_typing preamble_sub.g0 steps_sub
+    (ghost_comp preamble_sub.ctxt
+       (Tm_Star (list_as_vprop remaining_sub) Tm_Emp)) = coerce_eq steps_typing_sub () in
+
+  // matched_sub is emp, and list_as_vprop and vprop_as_list should cancel
+  let veq_sub : vprop_equiv preamble_sub.g
+    (comp_pre preamble_sub.c)
+    (Tm_Star (list_as_vprop unmatched_sub) matched_sub) = magic () in
+
+  assume (~ (Map.contains p.uvs y));
+  assert (~ (Map.contains p.ss y));
+  let uvs_sub = Map.upd p.uvs y t in
+  let ss_sub : substitution preamble_sub.g0 uvs_sub = p.ss in
+
+  assume (apply_ss ss_sub matched_sub == Tm_Emp);
+  let steps_typing_sub : st_typing preamble_sub.g0 steps_sub
+    (ghost_comp preamble_sub.ctxt
+       (Tm_Star (list_as_vprop remaining_sub) (apply_ss ss_sub matched_sub))) = coerce_eq steps_typing_sub () in
+
+  assume (~ (Set.mem y (dom_env preamble_sub.g0)));
+  assume (forall (x:var). Map.contains uvs_sub x ==>
+                          env_contains preamble_sub.g x (Map.sel uvs_sub x));
+  assume (dom_env preamble_sub.g ==
+          Set.union (dom_env preamble.g) (Set.singleton y));
+
+  let prover_state_sub : prover_state preamble_sub = {
+    matched = matched_sub;
+    unmatched = unmatched_sub;
+    remaining = remaining_sub;
+    steps = steps_sub;
+    uvs = uvs_sub;
+    ss = ss_sub;
+    remaining_typing;
+    unmatched_typing;
+    steps_typing = steps_typing_sub;
+    veq = veq_sub;
+    props = ();
+  } in
+  /////
+
+  // the function before this is Pure,
+  //   and it goes through quickly
+  // adding Tac steps below makes is real slow
+  let popt = prover prover_state_sub in
+  match popt with
+  | None -> None
+  | Some psub ->
+    // make sure witness is solved, and exists is uvars free
+    if Set.mem y (Map.domain psub.ss) &&
+       subset_bool (uvars (Tm_ExistsSL u t body) psub.uvs) (Map.domain psub.ss)
+    then begin
+      let steps_typing_sub : st_typing preamble_sub.g0 psub.steps
+        (ghost_comp
+           (list_as_vprop p.remaining)
+           (Tm_Star (list_as_vprop psub.remaining) (apply_ss psub.ss psub.matched))) = psub.steps_typing in
+      
+      let veq_sub : vprop_equiv preamble_sub.g
+        (comp_pre c_sub)
+        (Tm_Star (list_as_vprop []) psub.matched) = psub.veq in
+      // some manipulation of veq_sub
+      let veq_sub : vprop_equiv preamble_sub.g (comp_pre c_sub) psub.matched = magic () in
+      let veq_sub : vprop_equiv preamble_sub.g
+        (apply_ss psub.ss (comp_pre c_sub))
+        (apply_ss psub.ss psub.matched) =
+        veq_ss preamble_sub.g (comp_pre c_sub) psub.matched veq_sub psub.ss in
+
+      // THIS IS TODO, BUT WE SHOULD BE ABLE TO STRENGTHEN veq_sub to preamble_sub.g0
+      let veq_sub : vprop_equiv preamble_sub.g0
+        (apply_ss psub.ss (comp_pre c_sub))
+        (apply_ss psub.ss psub.matched) = magic () in
+
+      // use veq_sub on steps_typing_sub
+      let steps_typing_sub : st_typing preamble_sub.g0 psub.steps
+        (ghost_comp
+           (list_as_vprop p.remaining)
+           (Tm_Star (list_as_vprop psub.remaining) (apply_ss psub.ss (comp_pre c_sub)))) = magic () in
+
+      let t_typing_sub : st_typing preamble_sub.g t_sub c_sub = t_typing_sub in
+      assert (comp_post c_sub == Tm_ExistsSL u t body);
+
+      let t_typing_sub : st_typing preamble_sub.g
+        (apply_ss_st psub.ss t_sub)
+        (apply_c psub.ss c_sub) = typing_ss preamble_sub.g t_sub c_sub t_typing_sub psub.ss in
+
+      // AGAIN WE NEED A STRENGTHENING STEP HERE TO TAKE t_typing_sub to preamble_sub.g0
+      let t_typing_sub : st_typing preamble_sub.g0
+        (apply_ss_st psub.ss t_sub)
+        (apply_c psub.ss c_sub) = magic () in
+
+      assume (stateful_comp (apply_c psub.ss c_sub));
+      assume (comp_pre (apply_c psub.ss c_sub) == apply_ss psub.ss (comp_pre c_sub));
+      assume (comp_post (apply_c psub.ss c_sub) == apply_ss psub.ss (comp_post c_sub));
+
+      // g0 |- { p.remaining } psub.steps { psub.remaining * apply_ss psub.ss (comp_pre c_sub) }
+      // g0 |- { apply_ss psub.ss (comp_pre c_sub) } apply_ss_st psub.ss t_sub { apply_ss psub.ss (comp_post c_sub) }
+      // so we can bind these ... and note that c_sub is also ghost
+      let steps : st_term = magic () in  // Tm_Bind steps (apply_ss_st psub.ss t_sub)
+      let steps_c = ghost_comp (list_as_vprop p.remaining)
+                               (Tm_Star (list_as_vprop psub.remaining)
+                                        (apply_ss psub.ss (Tm_ExistsSL u t body))) in
+      let steps_typing : st_typing preamble_sub.g0 steps steps_c = magic () in  // bind typing
+      let steps_typing : st_typing preamble.g0 steps steps_c = steps_typing in
+
+      let psteps_typing : st_typing preamble.g0 p.steps
+        (ghost_comp preamble.ctxt
+                    (Tm_Star (list_as_vprop p.remaining)
+                             (apply_ss p.ss p.matched))) = p.steps_typing in
+
+      let ss_new : substitution preamble.g0 p.uvs = Map.restrict (Map.domain p.uvs) psub.ss in
+      assert (ss_new `ss_extends` p.ss);
+
+      // extends_apply psub.ss p.ss p.matched;
+
+      // let psteps_typing : st_typing preamble.g0 p.steps
+      //   (ghost_comp preamble.ctxt
+      //               (Tm_Star (list_as_vprop p.remaining)
+      //                        (apply_ss psub.ss p.matched))) = psteps_typing in
+      admit ()
+    end
+    else None
+
+
+// let has_no_uvars_from (t:term) (uvs:Set.set var) =
+//   freevars t `Set.disjoint` uvs
+
+// type uv_st =
+//   uvs:Set.set var & Map.t var (t:term { t `has_no_uvars_from` uvs})
+
+// let subst_uvs (t:term) (uvs:uv_st) : term = admit ()
+// let subst_uvs_st_term (t:st_term) (uvs:uv_st) : st_term = admit ()
+
+// noeq
+// type prover_state (g:env) (preamble:prover_state_preamble g) = {
+//   (* uvars and their solutions *)
+//   uv_st : uv_st;
+
+//   (* the in-progress proof state *)
+//   matched_pre:term; (* conjuncts that we have already derived *)
+//   unmatched_pre:list term; (* conjuncts remaining to be derived *)
+//   remaining_ctxt:list term; (* unused conjuncts in the context *)
+
+//   (* Ghost proof steps witnessing the derivation of matched_pre from ctxt *)
+//   proof_steps : st_term;
+
+//   ctxt_no_uvs : squash (
+//     preamble.ctxt `has_no_uvars_from` (dfst uv_st) /\
+//     list_as_vprop remaining_ctxt `has_no_uvars_from` (dfst uv_st)
+//   );
+
+//   proof_steps_typing:
+//     st_typing g
+//       (subst_uvs_st_term proof_steps uv_st)
+//       (ghost_comp preamble.ctxt (Tm_Star (subst_uvs (list_as_vprop remaining_ctxt) uv_st)
+//                                          (subst_uvs matched_pre uv_st)));
+
+//   pre_equiv:
+//     vprop_equiv g
+//       (subst_uvs (comp_pre preamble.c) uv_st)
+//       (Tm_Star (subst_uvs (list_as_vprop unmatched_pre) uv_st) (subst_uvs matched_pre uv_st));
+// }
+
+// let proof_steps_post (#g:_) (#preamble:_) (p:prover_state g preamble) : vprop =
+//   Tm_Star (list_as_vprop p.remaining_ctxt) (subst_uvs p.matched_pre p.uv_st)
+
+// let bind_proof_steps_with (#g:env) (#preamble:_) (p:prover_state g preamble)
+//   (t:st_term)
+//   (c:comp_st {comp_pre c == proof_steps_post p})
+//   (t_typing:st_typing g t c)
+//   : (t':st_term & st_typing g t' (comp_st_with_pre c preamble.ctxt))
+//   = admit()
+
+// type prover_step_t =
+//   #g:_ ->
+//   #preamble:_ ->
+//   p:prover_state g preamble ->
+//   T.Tac (option (prover_state g preamble))
+
+// //
+// // result of an intro (pure, exists, rewrite) step
+// //   that consumes some vprop v from p.unmatched_pre
+// //
+
+// let intro_comp (c:comp) =
+//   C_STGhost? c /\ comp_u c == u_zero /\ comp_res c == tm_unit
+
+// //
+// // A proof step that provides v, eating away some of the ctxt
+// //
+// noeq
+// type proof_step (g:env) (ctxt:list vprop) (v:vprop) = {
+//   remaining' : list vprop;
+
+//   t' : st_term;
+//   c' : c:comp { intro_comp c /\ comp_post c == v };
+//   t'_typing : st_typing g t' c';
+
+//   remaining_equiv : vprop_equiv g (list_as_vprop ctxt)
+//                                   (Tm_Star (comp_pre c') (list_as_vprop remaining'));
+// }
+
+// // An intro step that makes progress by solving one conjunct
+// // v from the p.unmatched_pre
+// noeq
+// type intro_from_unmatched_step (#g:env) (#preamble:_) (p:prover_state g preamble) = {
+//   uv_st : uv_st;
+
+//   v : vprop;
+
+//   // new unmatched pre and remaining ctxt
+//   remaining' : list vprop; 
+//   unmatched' : list vprop;
+
+//   t' : st_term;
+//   c' : c:comp { intro_comp c /\ comp_post c == v };
+//   t'_typing : st_typing g t' c';
  
-  // new unmatched pre and remaining ctxt
-  unmatched' : list vprop;
- 
-  // relation between new and old unmatched_pre and remaining_ctxt
-  unmatched_equiv : vprop_equiv g (list_as_vprop p.unmatched_pre)
-                                  (Tm_Star v (list_as_vprop unmatched'));
-}
+//   // relation between new and old unmatched_pre and remaining_ctxt
+//   unmatched_equiv : vprop_equiv g (list_as_vprop p.unmatched_pre)
+//                                   (Tm_Star v (list_as_vprop unmatched'));
+// }
 
-type proof_step_fn =
-  #g:_ ->
-  #ctxt:_ ->
-  #v:vprop ->
-  tot_typing g (list_as_vprop ctxt) Tm_VProp ->
-  tot_typing g v Tm_VProp ->
-  T.Tac (option (proof_step g ctxt v))
+// type proof_step_fn =
+//   #g:_ ->
+//   #ctxt:_ ->
+//   #v:vprop ->
+//   tot_typing g (list_as_vprop ctxt) Tm_VProp ->
+//   tot_typing g v Tm_VProp ->
+//   T.Tac (option (proof_step g ctxt v))
 
-type intro_from_unmatched_fn =
-  #g:_ ->
-  #preamble:_ ->
-  p:prover_state g preamble ->
-  T.Tac (option (intro_from_unmatched_step p))
+// type intro_from_unmatched_fn =
+//   #g:_ ->
+//   #preamble:_ ->
+//   p:prover_state g preamble ->
+//   T.Tac (option (intro_from_unmatched_step p))
 
-val apply_proof_step
-  (#g:env)
-  (#preamble:_)
-  (p:prover_state g preamble)
-  (v:vprop)
-  (r:proof_step g p.remaining_ctxt v)  
-  : T.Tac (p':prover_state g preamble {
-      p'.matched_pre == p.matched_pre /\
-      p'.unmatched_pre == p.unmatched_pre /\
-      p'.remaining_ctxt == v::r.remaining'
-    })
+// val apply_proof_step
+//   (#g:env)
+//   (#preamble:_)
+//   (p:prover_state g preamble)
+//   (v:vprop)
+//   (r:proof_step g p.remaining_ctxt v)  
+//   : T.Tac (p':prover_state g preamble {
+//       p'.matched_pre == p.matched_pre /\
+//       p'.unmatched_pre == p.unmatched_pre /\
+//       p'.remaining_ctxt == v::r.remaining'
+//     })
 
-val apply_intro_from_unmatched_step
-  (#g:env)
-  (#preamble:_)
-  (#p:prover_state g preamble)
-  (r:intro_from_unmatched_step p)
-  : T.Tac (p':prover_state g preamble {
-      p'.matched_pre == Tm_Star p.matched_pre r.v /\
-      p'.unmatched_pre == r.unmatched' /\
-      p'.remaining_ctxt == r.ps.remaining'
-    })
+// val apply_intro_from_unmatched_step
+//   (#g:env)
+//   (#preamble:_)
+//   (#p:prover_state g preamble)
+//   (r:intro_from_unmatched_step p)
+//   : T.Tac (p':prover_state g preamble {
+//       p'.matched_pre == Tm_Star p.matched_pre r.v /\
+//       p'.unmatched_pre == r.unmatched' /\
+//       p'.remaining_ctxt == r.ps.remaining'
+//     })
